Changed the structure of fairness preservation proof

fairness/lm_fairness_preservation.v
@@ -2,90 +2,12 @@ From stdpp Require Import option.
 From Paco Require Import paco1 paco2 pacotac.
 From trillium.program_logic Require Export adequacy.
 From trillium.fairness Require Export inftraces fairness fuel traces_match trace_utils.
-
-
-(* TODO: move? *)
-Lemma traces_match_LM_preserves_validity `{LM: LiveModel G M LSI}
-  `{C: Type} {L: Type}
-   (otr: trace C L) (auxtr : auxtrace (LM := LM))
-   state_rel lbl_rel outer_step :
-  traces_match lbl_rel state_rel outer_step LM.(lm_ls_trans) otr auxtr ->
-  auxtrace_valid auxtr (LM := LM).
-Proof.
-  revert otr auxtr. cofix CH. intros otr auxtr Hmatch.
-  inversion Hmatch; first by constructor.
-  constructor =>//. by eapply CH.
-Qed.
+From trillium.fairness Require Import lm_fair. (* TODO: remove? it's only for lm_lbl_matches_group *)
 
 
 Section fairness_preserved.
   Context `{LM: LiveModel G M LSI}.
   Context `{EqDecision G}.
-
-  (* State and labels of 'outer' model.
-     On top level it corresponds to the language. *)
-  (* TODO: formulate it in terms of actual model?
-     Possible for heap_lang but not clear how to do so for arbitrary language
-     (namely, how to uniformly define a state's set of live roles) *)
-  Context {So Lo: Type}.
-  Context `{EqDecision Lo}. 
-
-  Let out_trace := trace So (option Lo).
-
-  (* counterpart of locale step.
-     TODO: any restrictions? *)
-  Context (out_step: So -> option Lo -> So -> Prop). 
-
-  (* Representation of group labels on outer level *)
-  Context (lift_grole: G -> Lo).
-  Hypothesis (INJlg: Inj eq eq lift_grole). 
-  
-  Context (locale_prop: Lo -> So -> Prop).
-
-  (* Context (state_rel: cfg Λ → lm_ls LM → Prop). *)
-  Context (state_rel: So → lm_ls LM → Prop).
-
-  Definition lm_live_lift := forall ζ ρ δ c,
-      ls_mapping δ !! ρ = Some ζ ->
-      (* ρ ∈ live_roles _ δ ->  *)
-      state_rel c δ ->
-      (* locale_enabled ζ c *)
-      locale_prop (lift_grole ζ) c. 
-
-
-  Hypothesis (match_locale_prop_states: lm_live_lift).
-
-  Definition out_LM_labels_match (oζ : option Lo) (ℓ: lm_lbl LM) :=
-  match oζ with
-  | Some ζ =>
-      exists τ, ζ = lift_grole τ /\
-      match ℓ with
-      | Take_step _ τ' | Silent_step τ' => τ = τ'
-      | Config_step => False
-      end
-  | None => match ℓ with
-           | Config_step => True
-           | _ => False
-           end
-  end. 
-
-  (* TODO: rename *)
-  Definition lm_exaux_traces_match_gen: out_trace → auxtrace (LM := LM) → Prop :=
-    traces_match 
-    (* labels_match *) out_LM_labels_match
-    (* live_tids *) state_rel
-    (* locale_step  *) out_step
-    LM.(lm_ls_trans).
-
-  Lemma traces_match_labels tid ℓ c δ rex (raux : auxtrace (LM := LM)) :
-    lm_exaux_traces_match_gen (c -[Some tid]-> rex) (δ -[ℓ]-> raux) ->
-    exists τ, tid = lift_grole τ /\ 
-    ((∃ ρ, ℓ = Take_step ρ τ) ∨ (ℓ = Silent_step τ)).
-  Proof.
-    intros Hm. inversion Hm as [|?????? Hlab]; simplify_eq.
-    red in Hlab. destruct Hlab as [? [-> Hlab]]. 
-    destruct ℓ; eauto; inversion Hlab; simplify_eq; eauto.
-  Qed.
 
   Lemma mapping_live_role (δ: LiveState G M LSI) ρ:
     ρ ∈ M.(live_roles) δ ->
@@ -99,24 +21,22 @@ Section fairness_preserved.
   Local Hint Resolve mapping_live_role: core.
   Local Hint Resolve fuel_live_role: core.
 
-  Lemma match_locale_prop (extr : out_trace) (auxtr : auxtrace (LM := LM)) ζ ρ:
-    lm_exaux_traces_match_gen extr auxtr ->    
-    ls_mapping (trfirst auxtr) !! ρ = Some ζ ->
-    (* ρ ∈ live_roles _ (trfirst auxtr) -> *)
-    locale_prop (lift_grole ζ) (trfirst extr).
-  Proof.
-    intros Hm Hloc (* Hlive *).
-    eapply match_locale_prop_states; eauto.
-    eapply traces_match_first; eauto.  
-  Qed. 
-  
-  (* Local Hint Resolve match_locale_prop: core. *)
   Local Hint Resolve pred_first_trace: core.
 
+  (* TODO: fix names below *)
   
+  Definition group_step_or_dis
+    (τ: G) (δ: LiveState G M LSI) (oℓ: option (lm_lbl LM)) :=
+    (forall ρ, ¬ ls_mapping δ !! ρ = Some τ) \/ (∃ ℓ, oℓ = Some ℓ /\ lm_lbl_matches_group ℓ τ).
+
+  Definition fair_by_group auxtr τ n :=
+    pred_at auxtr n (λ δ _, exists ρ, ls_mapping δ !! ρ = Some τ) ->
+    ∃ m, pred_at auxtr (n + m)
+      (λ (δ : lm_ls LM) (ℓ : option (lm_lbl LM)), group_step_or_dis τ δ ℓ).
+
   Definition steps_or_unassigned 
     (ρ: fmrole M) (δ: LiveState G M LSI) (ℓ: option (lm_lbl LM)) :=
-    (∀ τ, ls_mapping δ !! ρ ≠ Some τ) \/ (∃ τ, ℓ = Some $ Take_step ρ τ).     
+    (∀ τ, ls_mapping δ !! ρ ≠ Some τ) \/ (∃ τ, ℓ = Some $ Take_step ρ τ).
     
   Definition fair_aux_SoU auxtr ρ n := 
     pred_at auxtr n (λ δ _, ρ ∈ dom (ls_mapping δ)) ->
@@ -136,59 +56,52 @@ Section fairness_preserved.
     rewrite -> (pred_at_sum _ n) in Hfair. rewrite Hafter in Hfair.
     destruct (Hfair Hpa) as (p&Hp).
     exists (p).
-    (* by rewrite <-Nat.add_assoc, ->!(pred_at_sum _ n), Hafter in Hp. *)
     rewrite <-Nat.add_assoc, ->!(pred_at_sum _ n) in Hp.
     by rewrite Hafter in Hp. 
   Qed.
 
-  Definition fairness_induction_stmt ρ fm f m τ extr (auxtr : auxtrace (LM := LM)) δ
+  Definition fairness_induction_stmt ρ fm f m τ (* extr *) (auxtr : auxtrace (LM := LM)) δ
     :=
-      (infinite_trace extr ->
-       (forall ζ, fair_by locale_prop ζ extr) ->
+      (
+        infinite_trace auxtr ->
+          (forall τ n, fair_by_group auxtr τ n) ->
        fm = (f, m) ->
-       lm_exaux_traces_match_gen extr auxtr ->
        δ = trfirst auxtr ->
        δ.(ls_fuel) !! ρ = Some f ->
        δ.(ls_mapping) !! ρ = Some τ ->
-       (pred_at extr m (λ c _, ¬locale_prop (lift_grole τ) c) ∨ 
-        pred_at extr m (λ _ oζ, oζ = Some (Some (lift_grole τ)))) ->
+       pred_at auxtr m (fun δ oℓ => group_step_or_dis τ δ oℓ)
+       ->
       ∃ M, pred_at auxtr M (fun δ ℓ => steps_or_unassigned ρ δ ℓ)). 
   
-  Local Lemma case1 ρ f m (extr': out_trace) (auxtr' : auxtrace (LM := LM)) δ ℓ :
+  Local Lemma case1 ρ f m (auxtr' : auxtrace (LM := LM)) δ ℓ :
     (∀ m0 : nat * nat,
          strict lt_lex m0 (f, m)
-         → ∀ (f m: nat) τ (extr : out_trace) (auxtr : auxtrace (LM := LM))
-             (δ : LiveState G M LSI), fairness_induction_stmt ρ m0 f m τ extr auxtr δ ) ->
+         → ∀ (f m: nat) τ (auxtr : auxtrace (LM := LM))
+             (δ : LiveState G M LSI),
+          auxtrace_valid auxtr -> fairness_induction_stmt ρ m0 f m τ (* extr *) auxtr δ ) ->
     (ρ ∈ dom (ls_fuel (trfirst auxtr')) → oless (ls_fuel (trfirst auxtr') !! ρ) (ls_fuel δ !! ρ)) ->
-    lm_exaux_traces_match_gen extr' auxtr' ->
-    infinite_trace extr' ->
+    auxtrace_valid auxtr' ->
+    infinite_trace auxtr' ->
     ls_fuel δ !! ρ = Some f ->
-    (∀ ζ, fair_by locale_prop ζ extr') ->
+    (forall τ n, fair_by_group auxtr' τ n) ->
     ∃ M0 : nat, pred_at (δ -[ ℓ ]-> auxtr') M0 (fun δ ℓ => steps_or_unassigned ρ δ ℓ).
-    Proof.
-      intros IH Hdec Hmatch Hinf Hsome Hfair.
+  Proof.
+      intros IH Hdec (* Hmatch *) Hvalid Hinf Hsome Hfair.
       unfold oless in Hdec.
       simpl in *.
       rewrite -> Hsome in *.
       destruct (ls_fuel (trfirst auxtr') !! ρ) as [f'|] eqn:Heq.
       -
-        
-        (* destruct (decide (ρ ∈ live_roles M (trfirst auxtr'))) as [Hρlive'|]; last first. *)
         destruct (decide (exists τ, ls_mapping (trfirst auxtr') !! ρ = Some τ)) as [MAP| ]; last first.
         { exists 1. apply pred_at_S.
           rewrite /steps_or_unassigned. apply pred_at_or. left.
           eapply pred_at_state_trfirst. eauto. }
-        (* have [τ' Hτ'] : is_Some (ls_mapping (trfirst auxtr') !! ρ) by eauto. *)
         destruct MAP as [τ' Hτ']. 
+        pose proof (Hfair τ' 0) as [p Hp]. 
+        { rewrite pred_at_state_trfirst. eauto. } 
 
-        have Hloc'en: pred_at extr' 0 (λ (c : So) (_ : option (option Lo)),
-                          locale_prop (lift_grole τ') c).
-        { rewrite /pred_at /= pred_first_trace.
-          eapply match_locale_prop; eauto. }
-
-        have [p Hp] := (Hfair (lift_grole τ') 0 Hloc'en).
         have [P Hind] : ∃ M0 : nat, pred_at auxtr' M0 (steps_or_unassigned ρ).
-        { eapply (IH _ _ _ p _ extr'); eauto.
+        { eapply (IH _ _ _ p _); eauto.
           Unshelve. unfold strict, lt_lex. specialize (Hdec ltac:(by eapply elem_of_dom_2)).
           lia. }
         exists (1+P). rewrite !pred_at_sum. simpl. done.
@@ -197,198 +110,199 @@ Section fairness_preserved.
         apply pred_at_state_trfirst.
         rewrite -ls_same_doms in Hdec.
         intros ??. apply Hdec, elem_of_dom. eauto. 
-    Qed.
+  Qed.
+  
+  Local Ltac SS' := eapply elem_of_dom; eauto. 
+  
+  (* TODO: use this lemma in other places *)
+  Lemma others_step_fuel_decr ρ f f' τ
+    δ ℓ δ'
+    (STEP: lm_ls_trans LM δ ℓ δ')
+    (Hfuel : ls_fuel δ !! ρ = Some f)
+    (Hmapping : ls_mapping δ !! ρ = Some τ)
+    (Hζ: ¬ lm_lbl_matches_group ℓ τ (LM := LM))
+    (FUEL: ls_fuel δ' !! ρ = Some f'):
+    f' ≤ f.
+  Proof.
+    simpl in *. destruct ℓ as [ρ0 ζ0| ζ0|]; try done.
+    + destruct STEP as (?&?&?&Hnoninc&?).
+      unfold fuel_must_not_incr in Hnoninc.
+      have Hneq: Some ρ ≠ Some ρ0 by congruence.
+      specialize (Hnoninc ρ ltac:(SS')).
+      unfold oleq in Hnoninc. rewrite Hfuel in Hnoninc.
+      rewrite FUEL in Hnoninc.
+      destruct Hnoninc as [?|[?|C]]. 
+      3: { destruct (proj1 C). eapply elem_of_dom; eauto. }
+      all: set_solver. 
+    + destruct STEP as (?&?&Hnoninc&?).
+      unfold fuel_must_not_incr in Hnoninc.
+      have Hneq: Some ρ ≠ None by congruence.
+      specialize (Hnoninc ρ ltac:(SS')).
+      unfold oleq in Hnoninc. rewrite Hfuel in Hnoninc.
+      rewrite FUEL in Hnoninc. 
+      destruct Hnoninc as [?|[?|C]]. 
+      3: { destruct (proj1 C). eapply elem_of_dom; eauto. }
+      all: set_solver.
+    + destruct STEP as [_ [_ [Hnoninc _]]].
+      have HnotNone: Some ρ ≠ None by congruence.
+      specialize (Hnoninc ρ ltac:(SS')).
+      unfold oleq in Hnoninc. rewrite Hfuel in Hnoninc.
+      rewrite FUEL in Hnoninc. 
+      destruct Hnoninc as [?|[?|C]]. 
+      3: { destruct (proj1 C). eapply elem_of_dom; eauto. }
+      all: set_solver.
+  Qed. 
+  
+  (* TODO: use this lemma in other places *)
+  Lemma owner_change_fuel_decr ρ f f'
+    δ ℓ δ'
+    τ τ''
+    (STEP: lm_ls_trans LM δ ℓ δ')
+    (Hfuel: ls_fuel δ !! ρ = Some f)
+    (Hmapping: ls_mapping δ !! ρ = Some τ)
+    (Hζ'' : ls_mapping δ' !! ρ = Some τ'')
+    (Hchange : τ ≠ τ'')
+    (FUEL: ls_fuel δ' !! ρ = Some f'):
+    f' < f.
+  Proof.
+    destruct ℓ as [ρ0 ζ0| ζ0|]; try done.
+    + destruct STEP as (?&?&Hdec&?&?).
+      unfold fuel_decr in Hdec. simplify_eq.
+      have Hmd: must_decrease ρ (Some ρ0) δ δ' (Some ζ0).
+      { econstructor 2. congruence. rewrite Hζ''; eauto. }
+      specialize (Hdec ρ ltac:(SS') ltac:(SS') Hmd).
+      unfold oleq in Hdec. rewrite Hfuel in Hdec.
+      by rewrite FUEL in Hdec. 
+    + destruct STEP as (?&Hdec&_).
+      unfold fuel_decr in Hdec. simplify_eq.
+      have Hmd: must_decrease ρ None δ δ' (Some ζ0).
+      { econstructor 2. congruence. rewrite Hζ''; eauto. }
+      specialize (Hdec ρ ltac:(SS') ltac:(SS') Hmd).
+      unfold oleq in Hdec. rewrite Hfuel in Hdec.
+      by rewrite FUEL in Hdec.
+    + destruct STEP as [_ [Hdec _]].
+      unfold fuel_decr in Hdec.
+      have Hmd: must_decrease ρ None δ δ' None.
+      { econstructor. congruence. rewrite Hζ''. eauto. }
+      specialize (Hdec ρ ltac:(SS') ltac:(SS') Hmd).
+      unfold oleq in Hdec. rewrite Hfuel in Hdec.
+      by rewrite FUEL in Hdec.
+  Qed.
 
-    Local Ltac SS' :=
-      (* epose proof ls_fuel_dom; *)
-      (* set_solver. *)
-      eapply elem_of_dom; eauto. 
-
-    Lemma others_step_fuel_decr ρ f f' τ
-      δ ℓ auxtr' 
-      c ζ' extr'
-      (Htm: lm_exaux_traces_match_gen (c -[ ζ' ]-> extr') (δ -[ ℓ ]-> auxtr'))
-      (Hfuel : ls_fuel δ !! ρ = Some f)
-      (Hmapping : ls_mapping δ !! ρ = Some τ)
-      (Hζ: Some (lift_grole τ) ≠ ζ')
-      (FUEL: ls_fuel (trfirst auxtr') !! ρ = Some f'):
-      f' ≤ f.
-    Proof.
-      inversion Htm as [|s1 ℓ1 r1 s2 ℓ2 r2 Hl Hs Hts Hls Hmatchrest]; simplify_eq.
-      destruct ζ' as [ζ'|]; last first; simpl in *.
-      - simpl in *. destruct ℓ; try done. destruct Hls as [_ [_ [Hnoninc _]]].
-        have HnotNone: Some ρ ≠ None by congruence.
-        specialize (Hnoninc ρ ltac:(SS')).
-        unfold oleq in Hnoninc. rewrite Hfuel in Hnoninc.
-        rewrite FUEL in Hnoninc. 
-        destruct Hnoninc as [?|[?|C]]. 
-        3: { destruct (proj1 C). eapply elem_of_dom; eauto. }
-        all: set_solver. 
-      - destruct Hl as [τ' [-> Hl]]. 
-        simpl in *. destruct ℓ as [ρ0 ζ0| ζ0|]; try done.
-        + destruct Hls as (?&?&?&Hnoninc&?).
-          unfold fuel_must_not_incr in Hnoninc.
-          have Hneq: Some ρ ≠ Some ρ0 by congruence.
-          specialize (Hnoninc ρ ltac:(SS')).
-          unfold oleq in Hnoninc. rewrite Hfuel in Hnoninc.
-          rewrite FUEL in Hnoninc.
-          destruct Hnoninc as [?|[?|C]]. 
-          3: { destruct (proj1 C). eapply elem_of_dom; eauto. }
-          all: set_solver. 
-        + destruct Hls as (?&?&Hnoninc&?).
-          unfold fuel_must_not_incr in Hnoninc.
-          have Hneq: Some ρ ≠ None by congruence.
-          specialize (Hnoninc ρ ltac:(SS')).
-          unfold oleq in Hnoninc. rewrite Hfuel in Hnoninc.
-          rewrite FUEL in Hnoninc. 
-          destruct Hnoninc as [?|[?|C]]. 
-          3: { destruct (proj1 C). eapply elem_of_dom; eauto. }
-          all: set_solver. 
-    Qed.
-    
-    Lemma owner_change_fuel_decr ρ f f'
-      c τ extr'
-      δ ℓ auxtr'
-      ζ' τ''
-      (Htm: lm_exaux_traces_match_gen (c -[ ζ' ]-> extr') (δ -[ ℓ ]-> auxtr'))
-      (Hfuel: ls_fuel δ !! ρ = Some f)
-      (Hmapping: ls_mapping δ !! ρ = Some τ)
-      (* (Hρlive: ρ ∈ live_roles M δ) *)
-      (* (Hρlive': ρ ∈ live_roles M (trfirst auxtr')) *)
-      (Hζ'' : ls_mapping (trfirst auxtr') !! ρ = Some τ'')
-      (Hchange : τ ≠ τ'')
-      (FUEL: ls_fuel (trfirst auxtr') !! ρ = Some f'):
-      f' < f.
-    Proof.
-      destruct ζ' as [ζ'|]; last first; simpl in *.
-      - inversion Htm as [|s1 ℓ1 r1 s2 ℓ2 r2 Hl Hs Hts Hls Hmatchrest]; simplify_eq.
-        simpl in *. destruct ℓ; try done. destruct Hls as [_ [Hdec _]].
-        unfold fuel_decr in Hdec.
-        have Hmd: must_decrease ρ None δ (trfirst auxtr') None.
-        { econstructor. congruence. rewrite Hζ''. eauto. }
-        specialize (Hdec ρ ltac:(SS') ltac:(SS') Hmd).
-        unfold oleq in Hdec. rewrite Hfuel in Hdec.
-        by rewrite FUEL in Hdec. 
-      - inversion Htm as [|s1 ℓ1 r1 s2 ℓ2 r2 Hl Hs Hts Hls Hmatchrest]; simplify_eq.
-        simpl in *.
-        destruct Hl as [τ' [-> Hl]]. 
-        destruct ℓ as [ρ0 ζ0| ζ0|]; try done.
-        + destruct Hls as (?&?&Hdec&?&?).
-          unfold fuel_decr in Hdec. simplify_eq.
-          have Hmd: must_decrease ρ (Some ρ0) δ (trfirst auxtr') (Some ζ0).
-          { econstructor 2. congruence. rewrite Hζ''; eauto. }
-          specialize (Hdec ρ ltac:(SS') ltac:(SS') Hmd).
-          unfold oleq in Hdec. rewrite Hfuel in Hdec.
-          by rewrite FUEL in Hdec. 
-        + destruct Hls as (?&Hdec&_).
-          unfold fuel_decr in Hdec. simplify_eq.
-          have Hmd: must_decrease ρ None δ (trfirst auxtr') (Some ζ0).
-          { econstructor 2. congruence. rewrite Hζ''; eauto. }
-          specialize (Hdec ρ ltac:(SS') ltac:(SS') Hmd).
-          unfold oleq in Hdec. rewrite Hfuel in Hdec.
-          by rewrite FUEL in Hdec. 
-    Qed.
-
+  (* TODO: move *)
+  Local Instance lm_lbl_match_Dec: 
+    forall ℓ τ, Decision (lm_lbl_matches_group ℓ τ (LM := LM)).
+  Proof.
+    intros. destruct ℓ; simpl; solve_decision.
+  Qed.
+  
+  (* TODO: get rid of it *)      
+  Lemma fair_by_group_after tr atr n
+    (AFTER: after n tr = Some atr)
+    (FG: ∀ τ n, fair_by_group tr τ n):
+    ∀ τ n, fair_by_group atr τ n.
+  Proof. 
+    intros. red. intros.
+    specialize (FG τ (n + n0)) as [k FAIR].
+    { eapply pred_at_sum; eauto. by rewrite AFTER. }
+    exists k.
+    rewrite -Nat.add_assoc Nat.add_comm in FAIR.
+    by rewrite pred_at_sum' AFTER in FAIR.
+  Qed. 
+  
+  (* TODO: get rid of it *)      
+  Lemma fair_by_group_cons δ ℓ tr
+    (FG: ∀ τ n, fair_by_group (δ -[ℓ]-> tr) τ n):
+    ∀ τ n, fair_by_group tr τ n.
+  Proof. 
+    intros.
+    eapply fair_by_group_after with (n := 1); eauto. done. 
+  Qed. 
 
   Lemma fairness_preserved_ind ρ:
-    ∀ fm f m τ (extr: out_trace) (auxtr: auxtrace (LM := LM)) δ,
-      fairness_induction_stmt ρ fm f m τ extr auxtr δ.
-  Proof.
+    ∀ fm f m τ (auxtr: auxtrace (LM := LM)) δ,
+      auxtrace_valid auxtr -> 
+      fairness_induction_stmt ρ fm f m τ auxtr δ.
+  Proof.    
     induction fm as [fm IH] using lex_ind.
-    intros f m τ extr auxtr δ Hexinfin Hfair -> Htm -> Hfuel Hmapping Hexen.
-    destruct extr as [|c ζ' extr'] eqn:Heq.
+    intros f m τ auxtr δ VALID Hexinfin Hfair -> Htm Hfuel Hmapping Hexen.
+    destruct auxtr as [|δ_ ℓ auxtr'] eqn:Heq.
     { have [??] := Hexinfin 1. done. }
-    have Hfair': (forall τ, fair_by locale_prop τ extr').
-    { intros. by eapply fair_by_cons. }
-    destruct auxtr as [|δ ℓ auxtr']; first by inversion Htm.
-    simpl in *. 
-    (* destruct (decide (ρ ∈ live_roles M δ)) as [Hρlive|]; last first. *)
-    (* { exists 0. left. unfold pred_at. simpl. intros contra. eauto. } *)
-    destruct (decide (Some (lift_grole τ) = ζ')) as [Hζ|Hζ].
-    - rewrite <- Hζ in *.
-      destruct (traces_match_labels _ _ _ _ _ _ Htm) as [τ' [LIFT_EQ Htm']].
-      apply INJlg in LIFT_EQ as <-. 
-      destruct Htm' as [[ρ' ->]| ->]; last first.
-      + inversion Htm as [|s1 ℓ1 r1 s2 ℓ2 r2 Hl Hs Hts Hls Hmatchrest]; simplify_eq.
-        unfold ls_trans in Hls. simpl in Hls. 
+    have Hfair': (forall τ n, fair_by_group auxtr' τ n). 
+    { eapply fair_by_group_cons; eauto. }
+    simpl in *. subst δ_. 
+    destruct (decide (lm_lbl_matches_group ℓ τ)) as [Hζ|Hζ].
+    - destruct ℓ; simpl in Hζ; try done; subst g; last first.       
+      + pose proof (auxtrace_valid_forall _ VALID 0) as Hls. 
+        simpl in Hls. 
         destruct Hls as (? & Hlsdec & Hlsincr).
         unfold fuel_decr in Hlsdec.
         have Hmustdec: must_decrease ρ None δ (trfirst auxtr') (Some τ).
         { constructor; eauto. }
         eapply case1 =>//.
         * move=> Hinfuel; apply Hlsdec => //; first set_solver.
+        * eapply auxtrace_valid_after with (n := 1); eauto. 
         * eapply infinite_cons =>//.
       + (* Three cases: *)
 (*            (1) ρ' = ρ and we are done *)
 (*            (2) ρ' ≠ ρ but they share the same ρ -> ρ decreases *)
 (*            (3) ρ' ≠ ρ and they don't have the same tid -> *)
 (*            impossible because tid and the label must match! *)
-        inversion Htm as [|s1 ℓ1 r1 s2 ℓ2 r2 Hl Hs Hts Hls Hmatchrest]; simplify_eq.
-        destruct (decide (ρ = ρ')) as [->|Hρneq].
+        pose proof (auxtrace_valid_forall _ VALID 0) as Hls. 
+        simpl in Hls. 
+        destruct (decide (ρ = f0)) as [->|Hρneq].
         { exists 0. right. rewrite /pred_at /=. eauto. }
         destruct Hls as (?&Hsame&Hdec&Hnotinc&_).
         rewrite -Hsame /= in Hmapping.
-        have Hmustdec: must_decrease ρ (Some ρ') δ (trfirst auxtr') (Some τ).
+        have Hmustdec: must_decrease ρ (Some f0) δ (trfirst auxtr') (Some τ).
         { constructor; eauto; congruence. }
         (* Copy and paste begins here *)
         eapply case1 =>//; last by eauto using infinite_cons.
+        2: { eapply auxtrace_valid_after with (n := 1); eauto. }
         intros Hinfuels. apply Hdec =>//. 
         clear -Hfuel. apply elem_of_dom; eauto.
 
     - (* Another thread is taking a step. *)
-      (* destruct (decide (ρ ∈ live_roles M (trfirst auxtr'))) as [Hρlive'|]; last first. *)
       destruct (decide (exists τ, ls_mapping (trfirst auxtr') !! ρ = Some τ)) as [MAP| ]; last first.
       { exists 1. apply pred_at_or. left.
         eapply pred_at_state_trfirst; eauto. }
       destruct m as [| m'].
-      { rewrite -> !pred_at_0 in Hexen. destruct Hexen as [Hexen|Hexen].
-        - exfalso. apply Hexen. eapply (match_locale_prop _ _ _ _ Htm); eauto. 
-        - simplify_eq. }
-      (* have [τ'' Hτ''] : is_Some (ls_mapping (trfirst auxtr') !! ρ) by eauto. *)
+      { rewrite -> !pred_at_0 in Hexen.
+        red in Hexen. destruct Hexen as [Hexen|Hexen].
+        -
+          exfalso. set_solver. 
+        - destruct Hexen as (?&?&?). set_solver. }
+      pose proof (auxtrace_valid_forall _ VALID 0) as Hls. simpl in Hls.
       destruct MAP as [τ'' Hτ'']. 
       destruct (ls_fuel (trfirst auxtr') !! ρ) as [f'| ] eqn:Hfuel'.
       2: { apply elem_of_dom_2 in Hτ''. apply not_elem_of_dom_2 in Hfuel'.
            rewrite ls_same_doms in Hτ''. done. }
       destruct (decide (τ = τ'')) as [<-|Hchange].
-      +
-        (* have [f' [Hfuel' Hff']] : exists f', ls_fuel (trfirst auxtr') !! ρ = Some f' ∧ f' ≤ f. *)
-        assert (f' <= f) as Hff' by (eapply others_step_fuel_decr; eauto).
-
+      + assert (f' <= f) as Hff' by (eapply others_step_fuel_decr; eauto).
         unfold fair_by in *.
-        have Hζ'en: pred_at extr' 0 (λ (c : So) _, locale_prop (lift_grole τ) c).
-        { rewrite /pred_at /= pred_first_trace.
-          eapply match_locale_prop; eauto. 
-          by inversion Htm. }
-
         have [P Hind] : ∃ M0 : nat, pred_at auxtr' M0 (steps_or_unassigned ρ).
-        { eapply (IH _ _ _ m' _ extr'); eauto. by eapply infinite_cons. by inversion Htm.
+        { eapply (IH _ _ _ m' _); eauto.
+          - eapply auxtrace_valid_after with (n := 1); eauto.
+          - by eapply infinite_cons.
           Unshelve. unfold strict, lt_lex. lia. }
         exists (1+P). rewrite !pred_at_sum. simpl. done.
-
-      +
-        assert (f' < f) as Hff' by (eapply owner_change_fuel_decr; eauto). 
-
+      + assert (f' < f) as Hff' by (eapply owner_change_fuel_decr; eauto). 
         unfold fair_by in *.
-        have: pred_at extr' 0 (λ c _, locale_prop (lift_grole τ'') c).
-        { rewrite /pred_at /= pred_first_trace.
-          eapply match_locale_prop; eauto. 
-          by inversion Htm. }
-        have Hζ'en: pred_at extr' 0 (λ c _, locale_prop (lift_grole τ'') c).
-        { rewrite /pred_at /= pred_first_trace.
-          eapply match_locale_prop; eauto. 
-          by inversion Htm. }
-        have [p Hp] := (Hfair' (lift_grole τ'') 0 Hζ'en).
+        pose proof (Hfair' τ'' 0) as [p Hp].
+        { rewrite pred_at_state_trfirst. eauto. }        
         have [P Hind] : ∃ M0 : nat, pred_at auxtr' M0 (steps_or_unassigned ρ).
-        { eapply (IH _ _ _ p _ extr'); eauto. by eapply infinite_cons. by inversion Htm.
+        { eapply (IH _ _ _ p _); eauto.
+          - eapply auxtrace_valid_after with (n := 1); eauto.
+          - by eapply infinite_cons.
           Unshelve. unfold strict, lt_lex. lia. }
         exists (1+P). rewrite !pred_at_sum. simpl. done.
   Qed.
-
   
-  Lemma exec_fairness_implies_step_or_unassign (extr: out_trace) (auxtr: auxtrace (LM := LM)):
-    infinite_trace extr ->
-    lm_exaux_traces_match_gen extr auxtr ->
-    (forall ζ, fair_by locale_prop ζ extr) ->
+  Lemma group_fairness_implies_step_or_unassign
+    (auxtr: auxtrace (LM := LM)):
+    infinite_trace auxtr ->
+    auxtrace_valid auxtr ->
+    (forall τ n, fair_by_group auxtr τ n) ->
     forall ρ n, fair_aux_SoU auxtr ρ n.
   Proof.
     intros Hinfin Hmatch Hex ρ n.
@@ -404,21 +318,19 @@ Section fairness_preserved.
     clear DOMn.
     have [f Hfuel] : is_Some((trfirst tr).(ls_fuel) !! ρ).
     { apply elem_of_dom. rewrite -ls_same_doms. eapply elem_of_dom; eauto. }
-    
-    have Hex' := Hex (lift_grole τ) n.
-    have [tr1' [Heq' Htr]] : exists tr1', after n extr = Some tr1' ∧ lm_exaux_traces_match_gen tr1' tr
-     by eapply traces_match_after.
-    have Hte: locale_prop (lift_grole τ) (trfirst tr1').
-    { eapply match_locale_prop; eauto. }
-    
-    setoid_rewrite pred_at_sum in Hex'. rewrite Heq' in Hex'.
-    have Hpa: pred_at extr n (λ c _, locale_prop (lift_grole τ) c).
-    { unfold pred_at. rewrite Heq'. destruct tr1'; eauto. }
-    destruct (Hex' Hpa) as [m Hm].
-    have ?: infinite_trace tr1'.
-    { have Hinf := infinite_trace_after n extr Hinfin. by rewrite Heq' in Hinf. }
-    eapply (fairness_preserved_ind ρ _ f m τ _ tr); eauto.
-    intros ?. by eapply fair_by_after.
+    have Hex' := Hex τ n.
+
+    red in Hex'. 
+    setoid_rewrite pred_at_sum in Hex'.
+    destruct Hex' as [m Hm].
+    { red. rewrite Heq. destruct tr; eauto. }
+
+    rewrite Heq in Hm.
+    have ?: infinite_trace tr.
+    { have Hinf := infinite_trace_after n auxtr Hinfin. by rewrite Heq in Hinf. }
+    eapply (fairness_preserved_ind ρ _ f m τ _); eauto.
+    - eapply auxtrace_valid_after; eauto. 
+    - eapply fair_by_group_after; eauto. 
   Qed.
 
   Lemma steps_or_unassigned_implies_aux_fairness (auxtr: auxtrace (LM := LM)):
@@ -432,21 +344,123 @@ Section fairness_preserved.
     apply pred_at_or in STEP. destruct STEP; eauto. left.
     eapply pred_at_impl; eauto. intros. simpl in *.
     intros [??]%mapping_live_role. congruence.
-  Qed.   
- 
-    
-  Theorem fairness_preserved (extr: out_trace) (auxtr: auxtrace (LM := LM)):
-    infinite_trace extr ->
-    lm_exaux_traces_match_gen extr auxtr ->
-    (forall ζ, fair_by locale_prop ζ extr) -> (forall ρ, fair_aux ρ auxtr (LM := LM)).
-  Proof.
-    intros.
-    apply steps_or_unassigned_implies_aux_fairness.
-    eapply exec_fairness_implies_step_or_unassign; eauto.
+  Qed.
+
+  Lemma group_fairness_implies_role_fairness (auxtr: auxtrace (LM := LM)):
+    infinite_trace auxtr ->
+    auxtrace_valid auxtr ->
+    (forall τ n, fair_by_group auxtr τ n) ->
+    (forall ρ, fair_aux ρ auxtr (LM := LM)).
+  Proof. 
+    intros. auto using steps_or_unassigned_implies_aux_fairness, 
+      group_fairness_implies_step_or_unassign.
   Qed. 
+    
+  Section Preservation.
+      Context {So Lo: Type}.
+      Context `{EqDecision Lo}. 
+
+      Let out_trace := trace So (option Lo).
+
+      (* counterpart of locale step.
+     TODO: any restrictions? *)
+      Context (out_step: So -> option Lo -> So -> Prop). 
+
+      (* Representation of group labels on outer level *)
+      Context (lift_grole: G -> Lo).
+      Hypothesis (INJlg: Inj eq eq lift_grole). 
+      
+      Context (locale_prop: Lo -> So -> Prop).
+
+      (* Context (state_rel: cfg Λ → lm_ls LM → Prop). *)
+      Context (state_rel: So → lm_ls LM → Prop).
+
+      Definition lm_live_lift := forall ζ ρ δ c,
+          ls_mapping δ !! ρ = Some ζ ->
+          (* ρ ∈ live_roles _ δ ->  *)
+          state_rel c δ ->
+          (* locale_enabled ζ c *)
+          locale_prop (lift_grole ζ) c. 
+
+
+      Hypothesis (match_locale_prop_states: lm_live_lift).
+
+      Definition out_LM_labels_match (oζ : option Lo) (ℓ: lm_lbl LM) :=
+        match oζ with
+        | Some ζ =>
+            exists τ, ζ = lift_grole τ /\
+                   match ℓ with
+                   | Take_step _ τ' | Silent_step τ' => τ = τ'
+                   | Config_step => False
+                   end
+        | None => match ℓ with
+                 | Config_step => True
+                 | _ => False
+                 end
+        end. 
+
+      (* TODO: rename *)
+      Definition lm_exaux_traces_match_gen: out_trace → auxtrace (LM := LM) → Prop :=
+        traces_match 
+          (* labels_match *) out_LM_labels_match
+          (* live_tids *) state_rel
+          (* locale_step  *) out_step
+          LM.(lm_ls_trans).
+
+      From trillium.fairness Require Import trace_lookup.
+
+      (* TODO: move *)
+      Lemma pred_at_impl {St L : Type} (P Q: St -> option L -> Prop)
+        (IMPL: forall s ol, P s ol -> Q s ol):
+        forall tr i, pred_at tr i P -> pred_at tr i Q.
+      Proof.
+        rewrite /pred_at. intros. 
+        destruct after; intuition; destruct t.
+        all: by apply IMPL.
+      Qed.
+    
+      Theorem fairness_preserved (extr: out_trace) (auxtr: auxtrace (LM := LM)):
+        infinite_trace extr ->
+        lm_exaux_traces_match_gen extr auxtr ->
+        (forall ζ, fair_by locale_prop ζ extr) -> (forall τ n, fair_by_group auxtr τ n).
+      Proof.
+        intros INF MATCH FAIR_OUT.
+        intros. red. intros ASG.
+        pose proof ASG as (δ & NTH & [ρ MAP])%pred_at_trace_lookup.        
+        edestruct @traces_match_state_lookup_2 as (c & ENTH & RELn); eauto.
+        
+        red in FAIR_OUT. edestruct FAIR_OUT as [m STEP].
+        { eapply pred_at_trace_lookup; eauto. }
+        apply pred_at_or in STEP.
+
+        apply pred_at_trace_lookup in STEP as (c' & ENTH' & STEP).
+        edestruct @traces_match_state_lookup_1 as (δ' & NTH' & RELn'); eauto. 
+        exists m. apply pred_at_trace_lookup. eexists. split; eauto.
+        red. destruct STEP as [EMP | STEP]. 
+        - eauto.
+        - right.
+          edestruct @traces_match_label_lookup_1 as (ℓ & NTH'l & LBL); eauto.
+          eexists. split; eauto. simpl in LBL.
+          destruct LBL as [? [->%INJlg ?]]. done. 
+      Qed.      
+      
+  End Preservation.
 
 End fairness_preserved.
 
+
+(* TODO: move? *)
+Lemma traces_match_LM_preserves_validity `{LM: LiveModel G M LSI}
+  `{C: Type} {L: Type}
+  (otr: trace C L) (auxtr : auxtrace (LM := LM))
+  state_rel lbl_rel outer_step :
+  traces_match lbl_rel state_rel outer_step LM.(lm_ls_trans) otr auxtr ->
+  auxtrace_valid auxtr (LM := LM).
+Proof.
+  revert otr auxtr. cofix CH. intros otr auxtr Hmatch.
+  inversion Hmatch; first by constructor.
+  constructor =>//. by eapply CH.
+Qed.
 
 Section lang_fairness_preserved.
   Context `{LM: LiveModel (locale Λ) M LSI}.
@@ -474,10 +488,12 @@ Section lang_fairness_preserved.
     lm_exaux_traces_match extr auxtr ->
     (forall ζ, fair_ex ζ extr) -> (forall ρ, fair_aux ρ auxtr (LM := LM)).
   Proof.
-    intros. eapply fairness_preserved; eauto.
+    intros. eapply group_fairness_implies_role_fairness; eauto. 
+    { eapply traces_match_infinite_trace; eauto. }
+    { eapply traces_match_LM_preserves_validity; eauto. }
+    eapply fairness_preserved; eauto.
     { apply _. }
     eapply match_locale_enabled_states_livetids; eauto.
-    Unshelve. apply _.
   Qed.
 
 End lang_fairness_preserved. 
@@ -509,8 +525,10 @@ Section model_fairness_preserved.
     lm_model_traces_match mtr auxtr ->
     (∀ ρ, fair_model_trace ρ mtr) -> (forall ρ, fair_aux ρ auxtr (LM := LM)).
   Proof.
-    intros. eapply fairness_preserved; eauto.
-    Unshelve. apply _.
+    intros. eapply group_fairness_implies_role_fairness; eauto. 
+    { eapply traces_match_infinite_trace; eauto. }
+    { eapply traces_match_LM_preserves_validity; eauto. }
+    eapply fairness_preserved; eauto.
   Qed.
 
 End model_fairness_preserved. 
